Refactor the impossible case proof

syntax.sig
@@ -1,15 +1,18 @@
 PTm(VarPTm) : Type
 PTag : Type
-Ty : Type
+BTag : Type
 
-Fun : Ty -> Ty -> Ty
-Prod : Ty -> Ty -> Ty
-Void : Ty
+nat : Type
 
 PL : PTag
 PR : PTag
+
+PPi : BTag
+PSig : BTag
 
 PAbs : (bind PTm in PTm) -> PTm
 PApp : PTm -> PTm -> PTm
 PPair : PTm -> PTm -> PTm
 PProj : PTag -> PTm -> PTm
+PBind : BTag -> PTm -> (bind PTm in PTm) -> PTm
+PUniv : nat -> PTm
