theories/fp_red.v
@@ -47,7 +47,13 @@ Module EPar.
     R a0 a1 ->
     R (PProj p a0) (PProj p a1)
   | VarTm i :
-    R (VarPTm i) (VarPTm i).
+    R (VarPTm i) (VarPTm i)
+  | Univ i :
+    R (PUniv i) (PUniv i)
+  | BindCong p A0 A1 B0 B1 :
+    R A0 A1 ->
+    R B0 B1 ->
+    R (PBind p A0 B0) (PBind p A1 B1).
 
   Lemma refl n (a : PTm n) : R a a.
   Proof.
@@ -126,6 +132,12 @@ with SN  {n} : PTm n -> Prop :=
   TRedSN a b ->
   SN b ->
   SN a
+| N_Bind p A B :
+  SN A ->
+  SN B ->
+  SN (PBind p A B)
+| N_Univ i :
+  SN (PUniv i)
 with TRedSN {n} : PTm n -> PTm n -> Prop :=
 | N_β a b :
   SN b ->
@@ -146,6 +158,63 @@ with TRedSN {n} : PTm n -> PTm n -> Prop :=
 
 Derive Dependent Inversion tred_inv with (forall n (a b : PTm n), TRedSN a b) Sort Prop.
 
+Definition ishf {n} (a : PTm n) :=
+  match a with
+  | PPair _ _ => true
+  | PAbs _ => true
+  | PUniv _ => true
+  | PBind _ _ _ => true
+  | _ => false
+  end.
+
+Definition ispair {n} (a : PTm n) :=
+  match a with
+  | PPair _ _ => true
+  | _ => false
+  end.
+
+Definition isabs {n} (a : PTm n) :=
+  match a with
+  | PAbs _ => true
+  | _ => false
+  end.
+
+Definition ishf_ren n m (a : PTm n)  (ξ : fin n -> fin m) :
+  ishf (ren_PTm ξ a) = ishf a.
+Proof. case : a => //=. Qed.
+
+Definition isabs_ren n m (a : PTm n)  (ξ : fin n -> fin m) :
+  isabs (ren_PTm ξ a) = isabs a.
+Proof. case : a => //=. Qed.
+
+Definition ispair_ren n m (a : PTm n)  (ξ : fin n -> fin m) :
+  ispair (ren_PTm ξ a) = ispair a.
+Proof. case : a => //=. Qed.
+
+
+Lemma PProj_imp n p a :
+  @ishf n a ->
+  ~~ ispair a ->
+  ~ SN (PProj p a).
+Proof.
+  move => + + h. move E  : (PProj p a) h => u h.
+  move : p a E.
+  elim : n u / h => //=.
+  hauto lq:on inv:SNe,PTm.
+  hauto lq:on inv:TRedSN.
+Qed.
+
+Lemma PAbs_imp n a b :
+  @ishf n a ->
+  ~~ isabs a ->
+  ~ SN (PApp a b).
+Proof.
+  move => + + h. move E : (PApp a b) h => u h.
+  move : a b E. elim  : n u /h=>//=.
+  hauto lq:on inv:SNe,PTm.
+  hauto lq:on inv:TRedSN.
+Qed.
+
 Lemma PProjAbs_imp n p (a : PTm (S n)) :
   ~ SN (PProj p (PAbs a)).
 Proof.
@@ -156,12 +225,32 @@ Proof.
   hauto lq:on inv:TRedSN.
 Qed.
 
-Lemma PProjPair_imp n (a b0 b1 : PTm n ) :
+Lemma PAppPair_imp n (a b0 b1 : PTm n ) :
   ~ SN (PApp (PPair b0 b1) a).
 Proof.
   move E : (PApp (PPair b0 b1) a) => u hu.
   move : a b0 b1 E.
   elim : n u / hu=>//=.
+  hauto lq:on inv:SNe.
+  hauto lq:on inv:TRedSN.
+Qed.
+
+Lemma PAppBind_imp n p (A : PTm n) B b :
+  ~ SN (PApp (PBind p A B) b).
+Proof.
+  move E :(PApp (PBind p A B) b) => u hu.
+  move : p A B b E.
+  elim : n u /hu=> //=.
+  hauto lq:on inv:SNe.
+  hauto lq:on inv:TRedSN.
+Qed.
+
+Lemma PProjBind_imp n p p' (A : PTm n) B :
+  ~ SN (PProj p (PBind p' A B)).
+Proof.
+  move E :(PProj p (PBind p' A B)) => u hu.
+  move : p p' A B E.
+  elim : n u /hu=>//=.
   hauto lq:on inv:SNe.
   hauto lq:on inv:TRedSN.
 Qed.
@@ -179,6 +268,8 @@ Fixpoint ne {n} (a : PTm n) :=
   | PAbs a => false
   | PPair _ _ => false
   | PProj _ a => ne a
+  | PUniv _ => false
+  | PBind _ _ _ => false
   end
 with nf {n} (a : PTm n) :=
   match a with
@@ -187,6 +278,8 @@ with nf {n} (a : PTm n) :=
   | PAbs a => nf a
   | PPair a b => nf a && nf b
   | PProj _ a => ne a
+  | PUniv _ => true
+  | PBind _ A B => nf A && nf B
 end.
 
 Lemma ne_nf n a : @ne n a -> nf a.
@@ -350,6 +443,8 @@ Proof.
     + sauto lq:on.
   - sauto lq:on.
   - sauto lq:on.
+  - sauto lq:on.
+  - sauto lq:on.
   - move => a b ha iha c h0.
     inversion h0; subst.
     inversion H1; subst.
@@ -410,7 +505,13 @@ Module RRed.
     R (PPair a b0) (PPair a b1)
   | ProjCong p a0 a1 :
     R a0 a1 ->
-    R (PProj p a0) (PProj p a1).
+    R (PProj p a0) (PProj p a1)
+  | BindCong0 p A0 A1 B :
+    R A0 A1 ->
+    R (PBind p A0 B) (PBind p A1 B)
+  | BindCong1 p A B0 B1 :
+    R B0 B1 ->
+    R (PBind p A B0) (PBind p A B1).
 
   Derive Dependent Inversion inv with (forall n (a b : PTm n), R a b) Sort Prop.
 
@@ -488,7 +589,13 @@ Module RPar.
     R a0 a1 ->
     R (PProj p a0) (PProj p a1)
   | VarTm i :
-    R (VarPTm i) (VarPTm i).
+    R (VarPTm i) (VarPTm i)
+  | Univ i :
+    R (PUniv i) (PUniv i)
+  | BindCong p A0 A1 B0 B1 :
+    R A0 A1 ->
+    R B0 B1 ->
+    R (PBind p A0 B0) (PBind p A1 B1).
 
   Lemma refl n (a : PTm n) : R a a.
   Proof.
@@ -581,6 +688,8 @@ Module RPar.
     | PPair a b => PPair (tstar a) (tstar b)
     | PProj p (PPair a b) => if p is PL then (tstar a) else (tstar b)
     | PProj p a => PProj p (tstar a)
+    | PUniv i => PUniv i
+    | PBind p A B => PBind p (tstar A) (tstar B)
     end.
 
   Lemma triangle n (a b : PTm n) :
@@ -609,6 +718,8 @@ Module RPar.
         elim /inv : ha => //=_ > ? ? [*]. subst.
         apply : ProjPair'; eauto using refl.
     - hauto lq:on ctrs:R inv:R.
+    - hauto lq:on ctrs:R inv:R.
+    - hauto lq:on ctrs:R inv:R.
   Qed.
 
   Lemma diamond n (a b c : PTm n) :
@@ -629,6 +740,8 @@ Proof.
   - hauto lq:on ctrs:SN inv:RPar.R.
   - hauto lq:on ctrs:SN.
   - hauto q:on ctrs:SN inv:SN, TRedSN'.
+  - hauto lq:on ctrs:SN inv:RPar.R.
+  - hauto lq:on ctrs:SN inv:RPar.R.
   - move => a b ha iha hb ihb.
     elim /RPar.inv : ihb => //=_.
     + move => a0 a1 b0 b1 ha0 hb0 [*]. subst.
@@ -649,91 +762,6 @@ Proof.
   - hauto lq:on inv:RPar.R ctrs:RPar.R, TRedSN', TRedSN.
   - sauto.
 Qed.
-
-Module EPar'.
-  Inductive R {n} : PTm n -> PTm n ->  Prop :=
-  (****************** Eta ***********************)
-  | AppEta a :
-    R (PAbs (PApp (ren_PTm shift a) (VarPTm var_zero))) a
-  | PairEta a :
-    R (PPair (PProj PL a) (PProj PR a)) a
-  (*************** Congruence ********************)
-  | AbsCong a0 a1 :
-    R a0 a1 ->
-    R (PAbs a0) (PAbs a1)
-  | AppCong0 a0 a1 b :
-    R a0 a1 ->
-    R (PApp a0 b) (PApp a1 b)
-  | AppCong1 a b0 b1 :
-    R b0 b1 ->
-    R (PApp a b0) (PApp a b1)
-  | PairCong0 a0 a1 b :
-    R a0 a1 ->
-    R (PPair a0 b) (PPair a1 b)
-  | PairCong1 a b0 b1 :
-    R b0 b1 ->
-    R (PPair a b0) (PPair a b1)
-  | ProjCong p a0 a1 :
-    R a0 a1 ->
-    R (PProj p a0) (PProj p a1).
-
-  Derive Dependent Inversion inv with (forall n (a b : PTm n), R a b) Sort Prop.
-
-  Lemma AppEta' n a (u : PTm n) :
-    u = (PAbs (PApp (ren_PTm shift a) (VarPTm var_zero))) ->
-    R u a.
-  Proof. move => ->. apply AppEta. Qed.
-
-  Lemma renaming n m (a b : PTm n) (ξ : fin n -> fin m) :
-    R a b -> R (ren_PTm ξ a) (ren_PTm ξ b).
-  Proof.
-    move => h. move : m ξ.
-    elim : n a b /h.
-
-    move => n a m ξ /=.
-    eapply AppEta'; eauto. by asimpl.
-    all : qauto ctrs:R.
-  Qed.
-
-  Lemma morphing_ren n m p (ρ0 ρ1 : fin n -> PTm m) (ξ : fin m -> fin p) :
-    (forall i, R (ρ0 i) (ρ1 i)) ->
-    (forall i, R ((funcomp (ren_PTm ξ) ρ0) i) ((funcomp (ren_PTm ξ) ρ1) i)).
-  Proof. eauto using renaming. Qed.
-
-End EPar'.
-
-Module EPars.
-
-  #[local]Ltac solve_s_rec :=
-  move => *; eapply rtc_l; eauto;
-         hauto lq:on ctrs:EPar'.R.
-
-  #[local]Ltac solve_s :=
-    repeat (induction 1; last by solve_s_rec); apply rtc_refl.
-
-  Lemma AbsCong n (a b : PTm (S n)) :
-    rtc EPar'.R a b ->
-    rtc EPar'.R (PAbs a) (PAbs b).
-  Proof. solve_s. Qed.
-
-  Lemma AppCong n (a0 a1 b0 b1 : PTm n) :
-    rtc EPar'.R a0 a1 ->
-    rtc EPar'.R b0 b1 ->
-    rtc EPar'.R (PApp a0 b0) (PApp a1 b1).
-  Proof. solve_s. Qed.
-
-  Lemma PairCong n (a0 a1 b0 b1 : PTm n) :
-    rtc EPar'.R a0 a1 ->
-    rtc EPar'.R b0 b1 ->
-    rtc EPar'.R (PPair a0 b0) (PPair a1 b1).
-  Proof. solve_s. Qed.
-
-  Lemma ProjCong n p (a0 a1  : PTm n) :
-    rtc EPar'.R a0 a1 ->
-    rtc EPar'.R (PProj p a0) (PProj p a1).
-  Proof. solve_s. Qed.
-
-End EPars.
 
 Module RReds.
 
@@ -766,6 +794,12 @@ Module RReds.
     rtc RRed.R (PProj p a0) (PProj p a1).
   Proof. solve_s. Qed.
 
+  Lemma BindCong n p (A0 A1 : PTm n) B0 B1 :
+    rtc RRed.R A0 A1 ->
+    rtc RRed.R B0 B1 ->
+    rtc RRed.R (PBind p A0 B0) (PBind p A1 B1).
+  Proof. solve_s. Qed.
+
   Lemma renaming n m (a b : PTm n) (ξ : fin n -> fin m) :
     rtc RRed.R a b -> rtc RRed.R (ren_PTm ξ a) (ren_PTm ξ b).
   Proof.
@@ -775,7 +809,7 @@ Module RReds.
   Lemma FromRPar n (a b : PTm n) (h : RPar.R a b) :
     rtc RRed.R a b.
   Proof.
-    elim : n a b /h; eauto using AbsCong, AppCong, PairCong, ProjCong, rtc_refl.
+    elim : n a b /h; eauto using AbsCong, AppCong, PairCong, ProjCong, rtc_refl, BindCong.
     move => n a0 a1 b0 b1 ha iha hb ihb.
     apply : rtc_r; last by apply RRed.AppAbs.
     by eauto using AppCong, AbsCong.
@@ -806,19 +840,6 @@ Proof.
   move : m ξ. elim : n / a => //=; solve [hauto b:on].
 Qed.
 
-Lemma ne_epar n (a b : PTm n) (h : EPar'.R a b ) :
-  (ne a -> ne b) /\ (nf a -> nf b).
-Proof.
-  elim : n a b /h=>//=; hauto qb:on use:ne_nf_ren, ne_nf.
-Qed.
-
-Definition ishf {n} (a : PTm n) :=
-  match a with
-  | PPair _ _ => true
-  | PAbs _ => true
-  | _ => false
-  end.
-
 Module NeEPar.
   Inductive R_nonelim {n} : PTm n -> PTm n ->  Prop :=
   (****************** Eta ***********************)
@@ -847,6 +868,12 @@ Module NeEPar.
     R_nonelim (PProj p a0) (PProj p a1)
   | VarTm i :
     R_nonelim (VarPTm i) (VarPTm i)
+  | Univ i :
+    R_nonelim (PUniv i) (PUniv i)
+  | BindCong p A0 A1 B0 B1 :
+    R_nonelim A0 A1 ->
+    R_nonelim B0 B1 ->
+    R_nonelim (PBind p A0 B0) (PBind p A1 B1)
   with R_elim {n} : PTm n -> PTm n -> Prop :=
   | NAbsCong a0 a1 :
     R_nonelim a0 a1 ->
@@ -863,7 +890,13 @@ Module NeEPar.
     R_elim a0 a1 ->
     R_elim (PProj p a0) (PProj p a1)
   | NVarTm i :
-    R_elim (VarPTm i) (VarPTm i).
+    R_elim (VarPTm i) (VarPTm i)
+  | NUniv i :
+    R_elim (PUniv i) (PUniv i)
+  | NBindCong p A0 A1 B0 B1 :
+    R_nonelim A0 A1 ->
+    R_nonelim B0 B1 ->
+    R_elim (PBind p A0 B0) (PBind p A1 B1).
 
   Scheme epar_elim_ind := Induction for R_elim Sort Prop
       with epar_nonelim_ind := Induction for R_nonelim Sort Prop.
@@ -881,6 +914,7 @@ Module NeEPar.
       qauto l:on inv:R_elim.
     - hauto lb:on.
     - hauto lq:on inv:R_elim.
+    - hauto b:on.
     - move => a0 a1 /negP ha' ha ih ha1.
       have {ih} := ih ha1.
       move => ha0.
@@ -897,6 +931,7 @@ Module NeEPar.
       move : ha h0. hauto lq:on inv:R_elim.
     - hauto lb: on drew: off.
     - hauto lq:on rew:off inv:R_elim.
+    - sfirstorder b:on.
   Qed.
 
   Lemma R_nonelim_nothf n (a b : PTm n) :
@@ -927,11 +962,17 @@ Module Type NoForbid.
 
   Axiom P_EPar : forall n (a b : PTm n), EPar.R a b -> P a -> P b.
   Axiom P_RRed : forall n (a b : PTm n), RRed.R a b -> P a -> P b.
-  Axiom P_AppPair : forall n (a b c : PTm n), ~ P (PApp (PPair a b) c).
-  Axiom P_ProjAbs : forall n p (a : PTm (S n)), ~ P (PProj p (PAbs a)).
+  (* Axiom P_AppPair : forall n (a b c : PTm n), ~ P (PApp (PPair a b) c). *)
+  (* Axiom P_ProjAbs : forall n p (a : PTm (S n)), ~ P (PProj p (PAbs a)). *)
+  (* Axiom P_ProjBind : forall n p p' (A : PTm n) B, ~ P (PProj p (PBind p' A B)). *)
+  (* Axiom P_AppBind : forall n p (A : PTm n) B b, ~ P (PApp (PBind p A B) b). *)
+  Axiom PAbs_imp : forall n a b, @ishf n a -> ~~ isabs a -> ~ P (PApp a b).
+  Axiom PProj_imp : forall  n p a, @ishf n a -> ~~ ispair a -> ~ P (PProj p a).
 
   Axiom P_AppInv : forall n (a b : PTm n), P (PApp a b) -> P a /\ P b.
   Axiom P_AbsInv : forall n (a : PTm (S n)), P (PAbs a) -> P a.
+  Axiom P_BindInv : forall n p (A : PTm n) B, P (PBind p A B) -> P A /\ P B.
+
   Axiom P_PairInv : forall n (a b : PTm n), P (PPair a b) -> P a /\ P b.
   Axiom P_ProjInv : forall n p (a : PTm n), P (PProj p a) -> P a.
   Axiom P_renaming : forall n m (ξ : fin n -> fin m) a , P (ren_PTm ξ a) <-> P a.
@@ -970,11 +1011,10 @@ Module SN_NoForbid <: NoForbid.
   Lemma P_RRed : forall n (a b : PTm n), RRed.R a b -> P a -> P b.
   Proof. hauto q:on use:red_sn_preservation, RPar.FromRRed. Qed.
 
-  Lemma P_AppPair : forall n (a b c : PTm n), ~ P (PApp (PPair a b) c).
-  Proof. sfirstorder use:PProjPair_imp. Qed.
-
-  Lemma P_ProjAbs : forall n p (a : PTm (S n)), ~ P (PProj p (PAbs a)).
-  Proof. sfirstorder use:PProjAbs_imp. Qed.
+  Lemma PAbs_imp : forall n a b, @ishf n a -> ~~ isabs a -> ~ P (PApp a b).
+    sfirstorder use:fp_red.PAbs_imp. Qed.
+  Lemma PProj_imp : forall  n p a, @ishf n a -> ~~ ispair a -> ~ P (PProj p a).
+    sfirstorder use:fp_red.PProj_imp. Qed.
 
   Lemma P_AppInv : forall n (a b : PTm n), P (PApp a b) -> P a /\ P b.
   Proof. sfirstorder use:SN_AppInv. Qed.
@@ -986,6 +1026,13 @@ Module SN_NoForbid <: NoForbid.
   Lemma P_ProjInv : forall n p (a : PTm n), P (PProj p a) -> P a.
   Proof. sfirstorder use:SN_ProjInv. Qed.
 
+  Lemma P_BindInv : forall n p (A : PTm n) B, P (PBind p A B) -> P A /\ P B.
+  Proof.
+    move => n p A B.
+    move E : (PBind p A B) => u hu.
+    move : p A B E. elim : n u /hu=>//=;sauto lq:on rew:off.
+  Qed.
+
   Lemma P_AbsInv : forall n (a : PTm (S n)), P (PAbs a) -> P a.
   Proof.
     move => n a. move E : (PAbs a) => u h.
@@ -996,13 +1043,19 @@ Module SN_NoForbid <: NoForbid.
   Lemma P_renaming : forall n m (ξ : fin n -> fin m) a , P (ren_PTm ξ a) <-> P  a.
   Proof. hauto lq:on use:sn_antirenaming, sn_renaming. Qed.
 
+  Lemma P_ProjBind : forall n p p' (A : PTm n) B, ~ P (PProj p (PBind p' A B)).
+  Proof. sfirstorder use:PProjBind_imp. Qed.
+
+  Lemma P_AppBind : forall n p (A : PTm n) B b, ~ P (PApp (PBind p A B) b).
+  Proof. sfirstorder use:PAppBind_imp. Qed.
+
 End SN_NoForbid.
 
 Module NoForbid_FactSN := NoForbid_Fact SN_NoForbid.
 
 Module UniqueNF (M : NoForbid) (MFacts : NoForbid_FactSig M).
   Import M MFacts.
-  #[local]Hint Resolve P_EPar P_RRed P_AppPair P_ProjAbs : forbid.
+  #[local]Hint Resolve P_EPar P_RRed PAbs_imp PProj_imp : forbid.
 
   Lemma η_split n (a0 a1 : PTm n) :
     EPar.R a0 a1 ->
@@ -1020,9 +1073,8 @@ Module UniqueNF (M : NoForbid) (MFacts : NoForbid_FactSig M).
       by eauto using RReds.renaming.
       apply NeEPar.AppEta=>//.
       sfirstorder use:NeEPar.R_nonelim_nothf.
-
-      case : b ih0 ih1 => //=.
-      + move => p ih0 ih1 _.
+      case /orP : (orbN (isabs b)).
+      + case : b ih0 ih1 => //= p ih0 ih1 _ _.
         set q := PAbs _.
         suff : rtc RRed.R q (PAbs p) by sfirstorder.
         subst q.
@@ -1033,16 +1085,14 @@ Module UniqueNF (M : NoForbid) (MFacts : NoForbid_FactSig M).
         apply : RRed.AbsCong => /=.
         apply RRed.AppAbs'. by asimpl.
       (* violates SN *)
-      + move => p p0 h. exfalso.
-        have : P (PApp (ren_PTm shift a0) (VarPTm var_zero))
-          by sfirstorder use:P_AbsInv.
-
-        have : rtc RRed.R (PApp (ren_PTm shift a0) (VarPTm var_zero))
-                 (PApp (ren_PTm shift (PPair p p0)) (VarPTm var_zero))
-          by hauto lq:on use:RReds.AppCong, RReds.renaming, rtc_refl.
-
-        move : P_RReds. repeat move/[apply] => /=.
-        hauto l:on use:P_AppPair.
+      + move /P_AbsInv in hP.
+        have {}hP : P (PApp (ren_PTm shift b) (VarPTm var_zero))
+          by sfirstorder use:P_RReds, RReds.AppCong, @rtc_refl, RReds.renaming.
+        move => ? ?.
+        have ? : ~~ isabs (ren_PTm shift b) by scongruence use:isabs_ren.
+        have ? : ishf (ren_PTm shift b) by scongruence use:ishf_ren.
+        exfalso.
+        sfirstorder use:PAbs_imp.
     - move => n a0 a1 h ih /[dup] hP.
       move /P_PairInv => [/P_ProjInv + _].
       move : ih => /[apply].
@@ -1051,16 +1101,9 @@ Module UniqueNF (M : NoForbid) (MFacts : NoForbid_FactSig M).
       exists (PPair (PProj PL b) (PProj PR b)).
       split. sfirstorder use:RReds.PairCong,RReds.ProjCong.
       hauto lq:on ctrs:NeEPar.R_nonelim use:NeEPar.R_nonelim_nothf.
-
-      case : b ih0 ih1 => //=.
-      (* violates SN *)
-      + move => p ?. exfalso.
-        have {}hP : P (PProj PL a0) by sfirstorder use:P_PairInv.
-        have : rtc RRed.R (PProj PL a0) (PProj PL (PAbs p))
-          by eauto using RReds.ProjCong.
-        move : P_RReds hP. repeat move/[apply] => /=.
-        sfirstorder use:P_ProjAbs.
-      + move => t0 t1 ih0 h1 _.
+      case /orP : (orbN (ispair b)).
+      + case : b ih0 ih1 => //=.
+        move => t0 t1 ih0 h1 _ _.
         exists (PPair t0 t1).
         split => //=.
         apply RReds.PairCong.
@@ -1068,6 +1111,12 @@ Module UniqueNF (M : NoForbid) (MFacts : NoForbid_FactSig M).
         apply RRed.ProjPair.
         apply : rtc_r; eauto using RReds.ProjCong.
         apply RRed.ProjPair.
+      + move => ? ?. exfalso.
+        move/P_PairInv : hP=>[hP _].
+        have : rtc RRed.R (PProj PL a0) (PProj PL b)
+          by eauto using RReds.ProjCong.
+        move : P_RReds hP. repeat move/[apply] => /=.
+        sfirstorder use:PProj_imp.
     - hauto lq:on ctrs:NeEPar.R_nonelim use:RReds.AbsCong, P_AbsInv.
     - move => n a0 a1 b0 b1 ha iha hb ihb.
       move => /[dup] hP /P_AppInv [hP0 hP1].
@@ -1076,8 +1125,9 @@ Module UniqueNF (M : NoForbid) (MFacts : NoForbid_FactSig M).
       case /orP : (orNb (ishf a2)) => [h|].
       + exists (PApp a2 b2). split; first by eauto using RReds.AppCong.
         hauto lq:on ctrs:NeEPar.R_nonelim use:NeEPar.R_nonelim_nothf.
-      + case : a2 iha0 iha1 => //=.
-        * move => p h0 h1 _.
+      + case /orP : (orbN (isabs a2)).
+        (* case : a2 iha0 iha1 => //=. *)
+        * case : a2 iha0 iha1 => //= p h0 h1 _ _.
           inversion h1; subst.
           ** exists (PApp a2 b2).
              split.
@@ -1087,11 +1137,9 @@ Module UniqueNF (M : NoForbid) (MFacts : NoForbid_FactSig M).
              hauto lq:on ctrs:NeEPar.R_nonelim.
           ** hauto lq:on ctrs:NeEPar.R_nonelim,NeEPar.R_elim use:RReds.AppCong.
         (* Impossible *)
-        * move => u0 u1 h. exfalso.
-          have : rtc RRed.R (PApp a0 b0) (PApp (PPair u0 u1) b0)
-            by hauto lq:on ctrs:rtc use:RReds.AppCong.
-          move : P_RReds hP; repeat move/[apply].
-          sfirstorder use:P_AppPair.
+        * move =>*. exfalso.
+          have : P (PApp a2 b0) by sfirstorder use:RReds.AppCong, @rtc_refl, P_RReds.
+          sfirstorder use:PAbs_imp.
     - hauto lq:on ctrs:NeEPar.R_nonelim use:RReds.PairCong, P_PairInv.
     - move => n p a0 a1 ha ih /[dup] hP /P_ProjInv.
       move : ih => /[apply]. move => [a2 [iha0 iha1]].
@@ -1100,13 +1148,13 @@ Module UniqueNF (M : NoForbid) (MFacts : NoForbid_FactSig M).
       split.  eauto using RReds.ProjCong.
       qauto l:on ctrs:NeEPar.R_nonelim, NeEPar.R_elim use:NeEPar.R_nonelim_nothf.
 
-      case : a2 iha0 iha1 => //=.
-      + move => u iha0. exfalso.
-        have : rtc RRed.R (PProj p a0) (PProj p (PAbs u))
+      case /orP : (orNb (ispair a2)).
+      + move => *. exfalso.
+        have : rtc RRed.R (PProj p a0) (PProj p a2)
           by sfirstorder use:RReds.ProjCong ctrs:rtc.
         move : P_RReds hP. repeat move/[apply].
-        sfirstorder use:P_ProjAbs.
-      + move => u0 u1 iha0 iha1 _.
+        sfirstorder use:PProj_imp.
+      + case : a2 iha0 iha1 => //= u0 u1 iha0 iha1 _ _.
         inversion iha1; subst.
         * exists (PProj p a2). split.
           apply : rtc_r.
@@ -1115,6 +1163,8 @@ Module UniqueNF (M : NoForbid) (MFacts : NoForbid_FactSig M).
           hauto lq:on ctrs:NeEPar.R_nonelim.
         * hauto lq:on ctrs:NeEPar.R_nonelim,NeEPar.R_elim use:RReds.ProjCong.
     - hauto lq:on ctrs:rtc, NeEPar.R_nonelim.
+    - hauto l:on.
+    - hauto lq:on ctrs:NeEPar.R_nonelim, rtc use:RReds.BindCong, P_BindInv.
   Qed.
 
 
